Core/Metatheory/Preservation.lean
@@ -2,163 +2,13 @@ import LeanSubst
 import Core.Term
 import Core.Reduction
 import Core.Typing
+import Core.Util
 
 import Core.Metatheory.Substitution
 import Core.Metatheory.Rename
+import Core.Metatheory.GlobalWf
 
 open LeanSubst
-
--- this means that the type of n.apply sp should be and arrow type
-theorem refl_spine_lemma :
-  OpenVarVal G n sp ->
-  ¬ (G&Δ, Γ ⊢ (g#n).apply sp : (A ~[K]~ B)) := by
-intro h j
-generalize tdef : (g#n).apply sp = t at *
-generalize Tdef : (A ~[K]~ B) = T at *
--- induction j <;> simp at *
-
-sorry
-
-theorem refl_is_val :
-  G&Δ, Γ ⊢ t : (A ~[K]~ B) ->
-  Value G t ->
-  ((t = refl! A) ∧ A = B) ∨ (∃ c1 c2, t = c1 `+ c2) := by
-intro j h; induction h
-any_goals (solve | cases j)
-case refl =>
-  cases j; constructor; simp
-case choice t1 t2 _ _ ih1 ih2 =>
-  cases j; apply Or.inr;  exists t1; exists t2
-case app ih =>
-  sorry
-
-
-theorem var_val_sound :
-  t.spine = some (x, sp) ->
-  is_stable x G ∨ OpenVarVal G x sp ->
-  ∀ t', ¬ G ⊢ t ~> t' := by
-intro h1 h2 t' r
-induction t generalizing x sp G
-any_goals (simp [Term.spine] at h1)
-case global =>
-  cases r;
-  case _ h2' _ _ _ _ _ h _ =>
-    simp [is_stable] at h2;   simp [Term.spine] at h
-    rcases h1 with ⟨e1, e2⟩; cases e1; cases e2; simp at *
-    rcases h with ⟨e1, e2⟩; cases e1; cases e2; simp at *
-    cases h2
-    case _ h =>
-      have lem := lookup_entry_openm_exists h2';
-      rcases lem with ⟨_, _, lem⟩
-      simp [is_ctor, is_instty] at h; rw[lem] at h
-      simp at h; simp [Entry.is_ctor, Entry.is_instty] at h
-    case _ h3 _ _ _ _ h =>
-      simp [OpenVarVal] at h;
-      rcases h with ⟨_, h⟩
-      replace h := h _ h3; omega
-  sorry -- exactly the same as above
-case ctor1 v _ ih =>
-  cases v <;> simp [Term.spine] at h1
-  rw[Option.bind_eq_some_iff] at h1; rcases h1 with ⟨_, h1, h2⟩; cases h2
-  cases r
-  all_goals (try simp [Term.spine] at h1)
-  case _ h _ =>
-    simp [Term.spine] at h; symm at h;
-    rw[Option.bind_eq_some_iff] at h; rcases h with ⟨_, h, e⟩; cases e
-    rw[h1] at h; cases h
-    simp [is_stable] at h2; case _ h2' _ _ _ _ _ =>
-    cases h2
-    case _ w _ _ _ _ _ _ _ _ _ h =>
-      have lem := @is_stable_implies_not_is_openm w.fst G (by simp [is_stable]; assumption)
-      apply lem h2'
-    case _ h3 _ _ h4 _ h =>
-      simp [OpenVarVal] at h
-      rcases h with ⟨_, h⟩
-      replace h :=  h _ h3
-      simp at h4; omega
-  case _ h => sorry
-  sorry
-case ctor2 v f _ ih1 ih2 =>
-  cases v <;> simp at *
-  all_goals (try simp [Term.spine] at h1)
-  case _ b =>
-    cases b <;> simp at *
-    case closed =>
-      cases r <;> try simp [Term.spine] at h1
-      case _ h _ =>
-        simp [Term.spine] at h; symm at h;
-        rw[Option.bind_eq_some_iff] at h; rcases h with ⟨w, h, e⟩; cases e
-        rcases h1 with ⟨_, e, h1⟩
-        rw[h1] at h; cases h
-        simp [is_stable] at h2; case _ h2' _ _ _ _ _ =>
-        cases h2
-        case _ w _ _ _ _ _ _ _ _ _ h =>
-          have lem := @is_stable_implies_not_is_openm x G (by simp [is_stable]; assumption)
-          apply lem h2'
-        case _ h3 _ _ h4 _ h =>
-          simp [OpenVarVal] at h
-          rcases h with ⟨_, h⟩
-          replace h :=  h _ h3
-          simp at h4; rw[e] at h; simp at h; omega
-      case _ h _ => sorry
-      all_goals (try case _ h _ => simp at h)
-      case _ h => sorry -- simp at h
-      sorry
-    case «open» =>
-      cases r <;> try simp [Term.spine] at h1
-      case _ h _ =>
-        simp [Term.spine] at h; symm at h;
-        rw[Option.bind_eq_some_iff] at h; rcases h with ⟨w, h, e⟩; cases e
-        rcases h1 with ⟨_, e, h1⟩
-        rw[h1] at h; cases h
-        simp [is_stable] at h2; case _ h2' _ _ _ _ _ =>
-        cases h2
-        case _ w _ _ _ _ _ _ _ _ _ h =>
-          have lem := @is_stable_implies_not_is_openm x G (by simp [is_stable]; assumption)
-          apply lem h2'
-        case _ h3 _ _ h4 _ h =>
-          simp [OpenVarVal] at h
-          rcases h with ⟨_, h⟩
-          replace h :=  h _ h3
-          simp at h4; rw[e] at h; simp at h; omega
-      case _ => sorry
-      case _ h _ => sorry
-      sorry
-      sorry
-      sorry
-
-
-theorem value_sound :
-  Value G t ->
-  t ≠ `0 ∧ ∀ t', ¬ G ⊢ t ~> t' := by
-intro h; induction h
-case _ =>
-  simp at *
-  constructor;
-  intro h; case _ tnf _ _ _ _  => rw[h] at tnf; simp [Term.spine] at tnf
-  case _ tnf _ _ h _ =>
-  apply var_val_sound (Eq.symm tnf); assumption
-all_goals (
-  case _ =>
-  apply And.intro; simp
-  intro t' r;
-  cases r <;> simp at *
-  try case right.ctor2_congr1 ih1 ih2 _ r _ =>
-      cases ih1; case _ h1 h2 =>
-      apply h2 _ r
-  try case right.ctor2_congr2 ih1 ih2 _ r _ =>
-      cases ih2; case _ h1 h2 =>
-      apply h2 _ r
-  try case _ h _ _ => simp [Term.spine] at h
-  try case _ h => simp [Term.spine] at h
-)
-
-theorem reduction_sound :
-  G ⊢ t ~> t' -> ¬ Value G t := by
-intro r v
-have lem := value_sound v
-rcases lem with ⟨_ , lem⟩
-apply lem t' r
 
 theorem instance_type_preservation :
   ⊢ G ->
@@ -170,10 +20,24 @@ sorry
 
 theorem lookup_defn_type_sound :
   ⊢ G ->
-  lookup_defn G x = .some t ->
-  G&Δ,Γ ⊢ t : T := by
-intro wf h1
-sorry
+  lookup x G = .some (Entry.defn y T t) ->
+  G&[],[] ⊢ t : T := by
+intro wf h
+induction G <;> simp [lookup] at *
+case _ hd tl ih =>
+  cases wf; case _ wfh wft =>
+  cases hd <;> simp [lookup] at *
+  case data =>
+    sorry
+  case opent => sorry
+  case openm => sorry
+  case defn => sorry
+  case inst => sorry
+  case instty =>
+    split at h
+    cases h
+    replace ih := ih wfh h
+    sorry
 
 theorem Typing.foldr_preservation :
   G&Δ ⊢ T : K ->
@@ -201,28 +65,33 @@ theorem preservation_prefix_match {p s t : Term} :
   G&Δ,Γ ⊢ t.apply ξ : T
 := by
 intro j1 j2 j3 j4 j5 j6 j7 j8
-induction s using Term.spine.induct generalizing x sp sp'
-case _ =>
-  simp [Term.spine] at j8; rcases j8 with ⟨j8, j9⟩
-  cases j8; cases j9
-  induction p using Term.spine.induct
-  case _ =>
-    simp [Term.spine] at j7; rcases j7 with ⟨j8, j9⟩
-    cases j8; cases j9
-    simp [prefix_equal] at j6; cases j6
-    simp [Term.apply]
-    sorry
-  simp [Term.spine] at j7; symm at j7
-  rw[Option.bind_eq_some_iff] at j7; rcases j7 with ⟨_, j7, j8⟩
-  sorry
-  sorry
-  sorry
-  sorry
+replace j6 := prefix_equal_law j6; subst j6
+have h7 := Term.apply_eq j7; subst h7
+replace j8 := Term.neutral_form_law j8; subst j8
+rw [Term.apply_spine_compose] at j2
+apply preservation_prefix_match_lemma (Eq.symm j7) j1 j2 j3 j4 j5
 
-sorry
-sorry
-sorry
-sorry
+-- induction s using Term.spine.induct generalizing x sp sp'
+-- case _ =>
+--   simp [Term.spine] at j8; rcases j8 with ⟨j8, j9⟩
+--   cases j8; cases j9
+--   induction p using Term.spine.induct
+--   case _ =>
+--     simp [Term.spine] at j7; rcases j7 with ⟨j8, j9⟩
+--     cases j8; cases j9
+--     simp [prefix_equal] at j6; cases j6
+--     simp [Term.apply]
+--     cases j1; cases j2; case _ j1 _ _ j2 => rw[j1] at j2; cases j2; sorry
+--   simp [Term.spine] at j7; symm at j7
+--   rw[Option.bind_eq_some_iff] at j7; rcases j7 with ⟨_, j7, j8⟩
+--   sorry
+--   sorry
+--   sorry
+--   sorry
+-- sorry
+-- sorry
+-- sorry
+-- sorry
 
 
 theorem preservation_lemma :
@@ -254,7 +123,7 @@ case global =>
   case defn h =>
     simp [Term.spine] at h; rcases h with ⟨e1, e2⟩; cases e1; cases e2;
     simp [Term.apply] at *
-    apply lookup_defn_type_sound wf; assumption
+    sorry -- apply lookup_defn_type_sound wf; assumption
 
 case mtch =>
   cases h
