Core/Metatheory/ValueSoundness.lean
@@ -1,0 +1,175 @@
+import LeanSubst
+import Core.Term
+import Core.Reduction
+import Core.Typing
+
+import Core.Metatheory.Substitution
+import Core.Metatheory.Rename
+
+-- this means that the type of n.apply sp should be and arrow type
+theorem refl_spine_lemma :
+  OpenVarVal G n sp ->
+  ¬ (G&Δ, Γ ⊢ (g#n).apply sp : (A ~[K]~ B)) := by
+intro h j
+generalize tdef : (g#n).apply sp = t at *
+generalize Tdef : (A ~[K]~ B) = T at *
+-- induction j <;> simp at *
+
+sorry
+
+theorem refl_is_val :
+  G&Δ, Γ ⊢ t : (A ~[K]~ B) ->
+  Value G t ->
+  ((t = refl! A) ∧ A = B) ∨ (∃ c1 c2, t = c1 `+ c2) := by
+intro j h; induction h
+any_goals (solve | cases j)
+case refl =>
+  cases j; constructor; simp
+case choice t1 t2 _ _ ih1 ih2 =>
+  cases j; apply Or.inr;  exists t1; exists t2
+case app ih =>
+  sorry
+
+
+theorem var_val_sound :
+  t.spine = some (x, sp) ->
+  is_stable x G ∨ OpenVarVal G x sp ->
+  ∀ t', ¬ G ⊢ t ~> t' := by
+intro h1 h2 t' r
+induction t generalizing x sp G
+any_goals (simp [Term.spine] at h1)
+case global =>
+  cases r;
+  case inst h2' _ _ _ _ _ h _ =>
+    simp [is_stable] at h2;   simp [Term.spine] at h
+    rcases h1 with ⟨e1, e2⟩; cases e1; cases e2; simp at *
+    rcases h with ⟨e1, e2⟩; cases e1; cases e2; simp at *
+    cases h2
+    case _ h =>
+      have lem := lookup_entry_openm_exists h2';
+      rcases lem with ⟨_, _, lem⟩
+      simp [is_ctor, is_instty] at h; rw[lem] at h
+      simp at h; simp [Entry.is_ctor, Entry.is_instty] at h
+    case _ h3 _ _ _ _ h =>
+      simp [OpenVarVal] at h;
+      rcases h with ⟨_, h⟩
+      replace h := h _ h3; omega
+  case defn e _ _ _ h3 h4 =>
+    cases h1.1; cases h1.2; clear h1
+    simp [Term.spine] at h4; cases h4.1; cases h4.2; clear h4
+    replace h3 := lookup_defn_is_defn_sound h3
+    cases h2
+    case _ h2 =>
+      replace h2 := is_stable_implies_not_is_defn h2
+      contradiction
+    case _ h =>
+      simp [OpenVarVal, is_openm] at h;
+      rcases h with ⟨h, _⟩
+      replace h3 := lookup_entry_defn_exists h3
+      rcases h3 with ⟨_, _, _, h3⟩
+      rw[h3] at h; simp [Entry.is_openm] at h
+case ctor1 v _ ih =>
+  cases v <;> simp [Term.spine] at h1
+  rw[Option.bind_eq_some_iff] at h1; rcases h1 with ⟨_, h1, h2⟩; cases h2
+  cases r
+  all_goals (try simp [Term.spine] at h1)
+  case inst h _ =>
+    simp [Term.spine] at h; symm at h;
+    rw[Option.bind_eq_some_iff] at h; rcases h with ⟨_, h, e⟩; cases e
+    rw[h1] at h; cases h
+    simp [is_stable] at h2; case _ h2' _ _ _ _ _ =>
+    cases h2
+    case _ w _ _ _ _ _ _ _ _ _ h =>
+      have lem := @is_stable_implies_not_is_openm w.fst G (by simp [is_stable]; assumption)
+      apply lem h2'
+    case _ h3 _ _ h4 _ h =>
+      simp [OpenVarVal] at h
+      rcases h with ⟨_, h⟩
+      replace h :=  h _ h3
+      simp at h4; omega
+  case defn h _ =>
+    sorry
+
+  sorry
+case ctor2 v f _ ih1 ih2 =>
+  cases v <;> simp at *
+  all_goals (try simp [Term.spine] at h1)
+  case _ b =>
+    cases b <;> simp at *
+    case closed =>
+      cases r <;> try simp [Term.spine] at h1
+      all_goals (try case _ h _ => simp at h)
+      case inst h _ =>
+        simp [Term.spine] at h; symm at h;
+        rw[Option.bind_eq_some_iff] at h; rcases h with ⟨w, h, e⟩; cases e
+        rcases h1 with ⟨_, e, h1⟩
+        rw[h1] at h; cases h
+        simp [is_stable] at h2; case _ h2' _ _ _ _ _ =>
+        cases h2
+        case _ w _ _ _ _ _ _ _ _ _ h =>
+          have lem := @is_stable_implies_not_is_openm x G (by simp [is_stable]; assumption)
+          apply lem h2'
+        case _ h3 _ _ h4 _ h =>
+          simp [OpenVarVal] at h
+          rcases h with ⟨_, h⟩
+          replace h :=  h _ h3
+          simp at h4; rw[e] at h; simp at h; omega
+      case defn h _ => sorry
+
+      case _ h => sorry -- simp at h
+      sorry
+    case «open» =>
+      cases r <;> try simp [Term.spine] at h1
+      case _ h _ =>
+        simp [Term.spine] at h; symm at h;
+        rw[Option.bind_eq_some_iff] at h; rcases h with ⟨w, h, e⟩; cases e
+        rcases h1 with ⟨_, e, h1⟩
+        rw[h1] at h; cases h
+        simp [is_stable] at h2; case _ h2' _ _ _ _ _ =>
+        cases h2
+        case _ w _ _ _ _ _ _ _ _ _ h =>
+          have lem := @is_stable_implies_not_is_openm x G (by simp [is_stable]; assumption)
+          apply lem h2'
+        case _ h3 _ _ h4 _ h =>
+          simp [OpenVarVal] at h
+          rcases h with ⟨_, h⟩
+          replace h :=  h _ h3
+          simp at h4; rw[e] at h; simp at h; omega
+      case _ => sorry
+      case _ h _ => sorry
+      sorry
+      sorry
+      sorry
+
+
+theorem value_sound :
+  Value G t ->
+  t ≠ `0 ∧ ∀ t', ¬ G ⊢ t ~> t' := by
+intro h; induction h
+case _ =>
+  simp at *
+  constructor;
+  intro h; case _ tnf _ _ _ _  => rw[h] at tnf; simp [Term.spine] at tnf
+  case _ tnf _ _ h _ =>
+  apply var_val_sound (Eq.symm tnf); assumption
+all_goals (
+  case _ =>
+  apply And.intro; simp
+  intro t' r;
+  cases r <;> simp at *
+  try case right.ctor2_congr1 ih1 ih2 _ r _ =>
+      cases ih1; case _ h1 h2 =>
+      apply h2 _ r
+  try case right.ctor2_congr2 ih1 ih2 _ r _ =>
+      cases ih2; case _ h1 h2 =>
+      apply h2 _ r
+  try case _ h _ _ => simp [Term.spine] at h
+  try case _ h => simp [Term.spine] at h
+)
+
+theorem reduction_sound :
+  G ⊢ t ~> t' -> ¬ Value G t := by
+intro r v
+have lem := value_sound v
+rcases lem with ⟨_ , lem⟩
+apply lem t' r
